src/opt/itree/iReorderStore.v
@@ -16,6 +16,7 @@ Require Import Configuration.
 Require Import Progress.
 
 Require Import FulfillStep.
+Require Import LowerPromises.
 
 Require Import SimMemory.
 Require Import SimPromises.
@@ -24,6 +25,7 @@ Require Import SimThread.
 Require Import iCompatibility.
 
 Require Import ReorderStep.
+Require Import ReorderAbortCommon.
 Require Import iProgressStep.
 
 Require Import ITreeLang.
@@ -35,13 +37,16 @@ Set Implicit Arguments.
 Inductive reorder_store l1 o1: forall R (i2:MemE.t R), Prop :=
 | reorder_store_load
     l2 o2
-    (ORD1: Ordering.le o1 Ordering.relaxed)
+    (ORD11: Ordering.le o1 Ordering.relaxed)
+    (ORD12: Ordering.le Ordering.plain o1)
     (ORD2: Ordering.le o2 Ordering.relaxed)
     (LOC: l1 <> l2):
     reorder_store l1 o1 (MemE.read l2 o2)
 | reorder_store_store
     l2 v2 o2
-    (ORD1: Ordering.le o1 Ordering.relaxed)
+    (ORD11: Ordering.le o1 Ordering.relaxed)
+    (ORD12: Ordering.le Ordering.plain o1)
+    (ORD2: Ordering.le Ordering.plain o2)
     (LOC: l1 <> l2):
     reorder_store l1 o1 (MemE.write l2 v2 o2)
 .
@@ -59,6 +64,25 @@ Inductive sim_store: forall R
     (FULFILL: fulfill_step lc1_src sc1_src l1 f1 t1 v1 None released1 o1 lc2_src sc2_src)
     (LOCAL: sim_local SimPromises.bot lc2_src lc1_tgt)
     (SC: TimeMap.le sc2_src sc1_tgt)
+    (MEMORY: sim_memory mem1_src mem1_tgt)
+    (WF_SRC: Local.wf lc1_src mem1_src)
+    (WF_TGT: Local.wf lc1_tgt mem1_tgt)
+    (SC_SRC: Memory.closed_timemap sc1_src mem1_src)
+    (SC_TGT: Memory.closed_timemap sc1_tgt mem1_tgt)
+    (MEM_SRC: Memory.closed mem1_src)
+    (MEM_TGT: Memory.closed mem1_tgt):
+    sim_store
+      (Vis i2 (fun v2 => Vis (MemE.write l1 v1 o1) (fun v1 => Ret (v1, v2)))) lc1_src sc1_src mem1_src
+      (Vis i2 (fun r => Ret (tt, r))) lc1_tgt sc1_tgt mem1_tgt
+| sim_store_racy_write
+    R
+    l1 v1 o1 (i2: MemE.t R)
+    lc1_src sc1_src mem1_src
+    lc1_tgt sc1_tgt mem1_tgt
+    (REORDER: reorder_store l1 o1 i2)
+    (RACY_WRITE: Local.racy_write_step lc1_src mem1_src l1 o1)
+    (LOCAL: sim_local SimPromises.bot lc1_src lc1_tgt)
+    (SC: TimeMap.le sc1_src sc1_tgt)
     (MEMORY: sim_memory mem1_src mem1_tgt)
     (WF_SRC: Local.wf lc1_src mem1_src)
     (WF_TGT: Local.wf lc1_tgt mem1_tgt)
@@ -95,8 +119,11 @@ Lemma sim_store_mon
              st_src lc_src sc2_src mem2_src
              st_tgt lc_tgt sc2_tgt mem2_tgt.
 Proof.
-  dependent destruction SIM1. exploit future_fulfill_step; try exact FULFILL; eauto; try refl.
-  i. des. econs; eauto.
+  dependent destruction SIM1.
+  - exploit future_fulfill_step; try exact FULFILL; eauto; try refl.
+    i. des. econs; eauto.
+  - exploit future_racy_write_step; try exact RACY_WRITE; eauto.
+    i. des. econs 2; eauto.
 Qed.
 
 Lemma sim_store_step
@@ -110,54 +137,137 @@ Lemma sim_store_step
                    st1_src lc1_src sc1_src mem1_src
                    st1_tgt lc1_tgt sc1_tgt mem1_tgt.
 Proof.
-  dependent destruction SIM. ii. right.
-  exploit fulfill_step_future; eauto; try viewtac. i. des.
-  inv STEP_TGT; [inv STEP|dependent destruction STEP; inv LOCAL0; ss; dependent destruction STATE; inv REORDER].
-  - (* promise *)
-    exploit Local.promise_step_future; eauto. i. des.
-    exploit sim_local_promise; try exact LOCAL0; (try by etrans; eauto); eauto. i. des.
-    exploit reorder_fulfill_promise; try exact FULFILL; try exact STEP_SRC; eauto. i. des.
-    exploit Local.promise_step_future; eauto. i. des.
-    esplits.
-    + ss.
-    + eauto.
-    + econs 2. econs 1. econs; eauto.
-    + auto.
-    + etrans; eauto.
-    + auto.
-    + right. econs; eauto.
-      eapply Memory.future_closed_timemap; eauto.
-  - (* load *)
-    exploit sim_local_read; try exact LOCAL0; (try by etrans; eauto); eauto; try refl. i. des.
-    exploit reorder_fulfill_read; try exact FULFILL; try exact STEP_SRC; eauto. i. des.
-    exploit Local.read_step_future; try exact STEP1; eauto. i. des.
-    exploit fulfill_write_sim_memory; eauto; try by viewtac. i. des.
-    esplits.
-    + ss.
-    + econs 2; eauto. econs.
-      * econs. econs 2. econs; [|econs 2]; eauto. econs. econs.
-      * auto.
-    + econs 2. econs 2. econs; [|econs 3]; eauto. econs; eauto.
-    + auto.
-    + auto.
-    + etrans; eauto.
-    + left. eapply paco11_mon; [apply sim_itree_ret|]; ss.
-  - (* store *)
-    hexploit sim_local_write_bot; try exact LOCAL1; eauto; try refl; try by viewtac. i. des.
-    hexploit reorder_fulfill_write_sim_memory; try exact FULFILL; try exact STEP_SRC; eauto; try by viewtac. i. des.
-    exploit Local.write_step_future; try exact STEP1; eauto; try by viewtac. i. des.
-    exploit fulfill_write_sim_memory; eauto; try by viewtac. i. des.
-    esplits.
-    + ss.
-    + econs 2; eauto. econs.
-      * econs. econs 2. econs; [|econs 3]; eauto. econs. econs.
-      * auto.
-    + econs 2. econs 2. econs; [|econs 3]; eauto. econs. econs.
-    + auto.
-    + etrans; eauto.
-    + etrans; eauto. etrans; eauto.
-    + left. eapply paco11_mon; [apply sim_itree_ret|]; ss.
-      etrans; eauto.
+  dependent destruction SIM.
+  { (* write *)
+    ii.
+    exploit fulfill_step_future; eauto; try viewtac. i. des.
+    inv STEP_TGT; [inv STEP|dependent destruction STEP; inv LOCAL0; ss; dependent destruction STATE; inv REORDER].
+    - (* promise *)
+      right.
+      exploit Local.promise_step_future; eauto. i. des.
+      exploit sim_local_promise; try exact LOCAL0; (try by etrans; eauto); eauto. i. des.
+      exploit reorder_fulfill_promise; try exact FULFILL; try exact STEP_SRC; eauto. i. des.
+      exploit Local.promise_step_future; eauto. i. des.
+      esplits.
+      + ss.
+      + eauto.
+      + econs 2. econs 1. econs; eauto.
+      + auto.
+      + etrans; eauto.
+      + auto.
+      + right. econs; eauto.
+        eapply Memory.future_closed_timemap; eauto.
+    - (* load *)
+      right.
+      exploit sim_local_read; try exact LOCAL0; (try by etrans; eauto); eauto; try refl. i. des.
+      exploit reorder_fulfill_read; try exact FULFILL; try exact STEP_SRC; eauto. i. des.
+      exploit Local.read_step_future; try exact STEP1; eauto. i. des.
+      exploit fulfill_write_sim_memory; eauto; try by viewtac. i. des.
+      esplits.
+      + ss.
+      + econs 2; eauto. econs.
+        * econs. econs 2. econs; [|econs 2]; eauto. econs. econs.
+        * auto.
+      + econs 2. econs 2. econs; [|econs 3]; eauto. econs; eauto.
+      + auto.
+      + auto.
+      + etrans; eauto.
+      + left. eapply paco11_mon; [apply sim_itree_ret|]; ss.
+    - (* store *)
+      right.
+      hexploit sim_local_write_bot; try exact LOCAL1;
+        try match goal with
+            | [|- is_true (Ordering.le _ _)] => refl
+            end; eauto; try refl; try by viewtac. i. des.
+      hexploit reorder_fulfill_write_sim_memory; try exact FULFILL; try exact STEP_SRC; eauto; try by viewtac. i. des.
+      exploit Local.write_step_future; try exact STEP1; eauto; try by viewtac. i. des.
+      exploit fulfill_write_sim_memory; eauto; try by viewtac. i. des.
+      esplits.
+      + ss.
+      + econs 2; eauto. econs.
+        * econs. econs 2. econs; [|econs 3]; eauto. econs. econs.
+        * auto.
+      + econs 2. econs 2. econs; [|econs 3]; eauto. econs. econs.
+      + auto.
+      + etrans; eauto.
+      + etrans; eauto. etrans; eauto.
+      + left. eapply paco11_mon; [apply sim_itree_ret|]; ss.
+        etrans; eauto.
+    - (* na write *)
+      inv LOCAL1. destruct ord; ss.
+    - (* racy read *)
+      right.
+      exploit sim_local_racy_read; try exact LOCAL1; eauto; try refl. i. des.
+      exploit reorder_fulfill_racy_read; try exact FULFILL; eauto. i. des.
+      exploit fulfill_write_sim_memory; eauto. i. des.
+      esplits.
+      + ss.
+      + econs 2; eauto. econs.
+        * econs. econs 2. econs; [|econs 9]; eauto. econs. econs.
+        * auto.
+      + econs 2. econs 2. econs; [|econs 3]; eauto. econs. ss.
+      + auto.
+      + ss.
+      + etrans; eauto.
+      + left. eapply paco11_mon; [apply sim_itree_ret|]; ss.
+    - (* racy write *)
+      left.
+      exploit sim_local_racy_write; try exact LOCAL1;
+        try match goal with
+            | [|- is_true (Ordering.le _ _)] => refl
+            end; eauto; try refl. i. des.
+      exploit reorder_fulfill_racy_write; try exact FULFILL; eauto. i. des.
+      unfold Thread.steps_failure.
+      esplits; try refl.
+      + econs 2. econs; [|econs 10]; eauto. econs. econs.
+      + ss.
+  }
+
+  { (* racy write *)
+    ii. left. unfold Thread.steps_failure.
+    inv REORDER.
+    - (* load *)
+      exploit progress_read_step_cur; try exact WF_SRC; eauto. i. des.
+      exploit read_step_cur_future; try exact READ; eauto. i. des.
+      esplits.
+      + econs 2; try refl. econs.
+        * econs. econs 2. econs; [|econs 2]; eauto. econs. econs.
+        * ss.
+      + econs 2. econs; [|econs 10].
+        * econs. econs.
+        * inv RACY_WRITE. econs; eauto; try congr.
+          { inv RACE. econs. congr. }
+          { ii. rewrite <- PROMISES, <- TVIEW in *. eauto. }
+      + ss.
+    - (* store *)
+      exploit (@LowerPromises.steps_promises_rel
+                 (lang (() * ()))
+                 (Thread.mk (lang (() * ()))
+                            (Vis (MemE.write l2 v2 o2) (fun v0 : () => Vis (MemE.write l1 v1 o1) (fun v3 : () => Ret (v3, v0))))
+                            lc1_src sc1_src mem1_src)); s; eauto.
+      i. des. destruct e2. ss.
+      exploit LowerPromises.rtc_opt_promise_step_future; eauto. s. i. des. subst.
+      hexploit LowerPromises.promises_rel_promise_consistent; try apply RACY_WRITE; eauto. i.
+      hexploit LowerPromises.promises_rel_nonsynch; eauto. i.
+      exploit Thread.rtc_tau_step_future; try exact STEPS0; eauto. s. i. des.
+      exploit write_step_consistent; try exact WF2; eauto. i. des.
+      esplits.
+      + eapply rtc_n1; eauto. econs.
+        * econs. econs 2. econs; [|econs 3; eauto]. econs. econs.
+        * ss.
+      + econs 2. econs; [|econs 10].
+        * econs. econs.
+        * inv RACY_WRITE.
+          exploit Thread.rtc_tau_step_non_promised; try exact STEPS0; eauto. s. i. des.
+          exploit Local.program_step_non_promised; [econs 3|..]; try exact STEP; eauto. i. des.
+          econs; eauto; try congr.
+          inv RACE. econs. rewrite TVIEW in TS.
+          inv STEP. ss.
+          apply TimeFacts.join_spec_lt; auto.
+          unfold TimeMap.singleton, Loc.LocFun.add, Loc.LocFun.init, Loc.LocFun.find. condtac; ss.
+          eapply TimeFacts.le_lt_lt; eauto. apply Time.bot_spec.
+      + ss.
+  }
 Qed.
 
 Lemma sim_store_sim_thread R:
@@ -166,39 +276,79 @@ Proof.
   pcofix CIH. i. pfold. ii. ss. splits; ss; ii.
   - inv TERMINAL_TGT. inv PR; ss.
   - exploit sim_store_mon; eauto. i.
-    dup x0. dependent destruction x1. subst.
-    exploit (progress_program_step_non_update i2 (fun r => Ret (tt, r))); eauto.
-    { dependent destruction PR. inv REORDER0; ss. }
-    i. des.
-    destruct th2.
-    exploit sim_store_step; eauto.
-    { econs 2. eauto. }
-    i. des; eauto.
-    + exploit program_step_promise; eauto. i.
-      exploit Thread.rtc_tau_step_future; eauto. s. i. des.
-      exploit Thread.opt_step_future; eauto. s. i. des.
-      exploit Thread.program_step_future; eauto. s. i. des.
-      punfold SIM. exploit SIM; try apply SC3; eauto; try refl.
-      { exploit Thread.program_step_promises_bot; eauto. s. i.
-        eapply Local.bot_promise_consistent; eauto. }
-      s. i. des.
-      exploit PROMISES; eauto. i. des.
-      * left.
-        unfold Thread.steps_failure in *. des.
-        esplits; [|eauto].
-        etrans; eauto. etrans; [|eauto].
-        inv STEP_SRC; eauto. econs 2; eauto. econs; eauto.
-        { econs. eauto. }
-        { etrans; eauto.
-          destruct e; by inv STEP; ss; dependent destruction STATE; inv REORDER. }
-      * right.
-        esplits; [|eauto].
-        etrans; eauto. etrans; [|eauto].
-        inv STEP_SRC; eauto. econs 2; eauto. econs; eauto.
-        { econs. eauto. }
-        { etrans; eauto.
-          destruct e; by inv STEP; ss; dependent destruction STATE; inv REORDER. }
-    + destruct SIM. dependent destruction STEP; ss; dependent destruction STATE. destruct e; ss.
+    dup x0. dependent destruction x1.
+    { subst.
+      exploit (progress_program_step_non_update i2 (fun r => Ret (tt, r))); eauto.
+      { dependent destruction PR; inv REORDER0; ss. }
+      i. des.
+      destruct th2.
+      exploit sim_store_step; eauto.
+      { econs 2. eauto. }
+      i. des; eauto.
+      + exploit Thread.program_step_promises_bot; eauto. s. i.
+        exploit Thread.rtc_tau_step_future; eauto. s. i. des.
+        exploit Thread.opt_step_future; eauto. s. i. des.
+        exploit Thread.program_step_future; eauto. s. i. des.
+        punfold SIM. exploit SIM; try apply SC3; eauto; try refl.
+        { exploit Thread.program_step_promises_bot; eauto. s. i.
+          eapply Local.bot_promise_consistent; eauto. }
+        s. i. des.
+        exploit PROMISES; eauto. i. des.
+        * left.
+          unfold Thread.steps_failure in *. des.
+          esplits; [|eauto|]; ss.
+          etrans; eauto. etrans; [|eauto].
+          inv STEP_SRC; eauto. econs 2; eauto. econs; eauto.
+          { econs. eauto. }
+          { etrans; eauto.
+            destruct e; by inv STEP; ss; dependent destruction STATE; inv REORDER. }
+        * right.
+          esplits; [|eauto].
+          etrans; eauto. etrans; [|eauto].
+          inv STEP_SRC; eauto. econs 2; eauto. econs; eauto.
+          { econs. eauto. }
+          { etrans; eauto.
+            destruct e; by inv STEP; ss; dependent destruction STATE; inv REORDER. }
+      + destruct SIM.
+        { dependent destruction STEP; ss; dependent destruction STATE. destruct e; ss. }
+        { dependent destruction STEP; ss; dependent destruction STATE. destruct e; ss. }
+    }
+    { subst.
+      exploit (progress_program_step_non_update i2 (fun r => Ret (tt, r))); eauto.
+      { dependent destruction PR; inv REORDER0; ss. }
+      i. des.
+      destruct th2.
+      exploit sim_store_step; eauto.
+      { econs 2. eauto. }
+      i. des; eauto.
+      + exploit Thread.program_step_promises_bot; eauto. s. i.
+        exploit Thread.rtc_tau_step_future; eauto. s. i. des.
+        exploit Thread.opt_step_future; eauto. s. i. des.
+        exploit Thread.program_step_future; eauto. s. i. des.
+        punfold SIM. exploit SIM; try apply SC3; eauto; try refl.
+        { exploit Thread.program_step_promises_bot; eauto. s. i.
+          eapply Local.bot_promise_consistent; eauto. }
+        s. i. des.
+        exploit PROMISES; eauto. i. des.
+        * left.
+          unfold Thread.steps_failure in *. des.
+          esplits; [|eauto|]; ss.
+          etrans; eauto. etrans; [|eauto].
+          inv STEP_SRC; eauto. econs 2; eauto. econs; eauto.
+          { econs. eauto. }
+          { etrans; eauto.
+            destruct e; by inv STEP; ss; dependent destruction STATE; inv REORDER. }
+        * right.
+          esplits; [|eauto].
+          etrans; eauto. etrans; [|eauto].
+          inv STEP_SRC; eauto. econs 2; eauto. econs; eauto.
+          { econs. eauto. }
+          { etrans; eauto.
+            destruct e; by inv STEP; ss; dependent destruction STATE; inv REORDER. }
+      + destruct SIM.
+        { dependent destruction STEP; ss; dependent destruction STATE. destruct e; ss. }
+        { dependent destruction STEP; ss; dependent destruction STATE. destruct e; ss. }
+    }
   - exploit sim_store_mon; eauto. i. des.
     exploit sim_store_step; eauto. i. des; eauto.
     + right. esplits; eauto.
